wjirbgijere

.lake/build/ir/Games/gameLib_fixfix/Zermelo.c
@@ -1,0 +1,192 @@
+// Lean compiler output
+// Module: Games.gameLib_fixfix.Zermelo
+// Imports: Init Games.gameLib_fixfix.Termination
+#include <lean/lean.h>
+#if defined(__clang__)
+#pragma clang diagnostic ignored "-Wunused-parameter"
+#pragma clang diagnostic ignored "-Wunused-label"
+#elif defined(__GNUC__) && !defined(__CLANG__)
+#pragma GCC diagnostic ignored "-Wunused-parameter"
+#pragma GCC diagnostic ignored "-Wunused-label"
+#pragma GCC diagnostic ignored "-Wunused-but-set-variable"
+#endif
+#ifdef __cplusplus
+extern "C" {
+#endif
+LEAN_EXPORT lean_object* l_Hist__from__moves(lean_object*);
+LEAN_EXPORT lean_object* l_moves__from__strats(lean_object*, lean_object*);
+LEAN_EXPORT lean_object* l_Hist__from__moves___rarg(lean_object*, lean_object*);
+lean_object* l_List_get___rarg(lean_object*, lean_object*);
+LEAN_EXPORT lean_object* l_List_rget___rarg___boxed(lean_object*, lean_object*);
+lean_object* l_List_mapTR_loop___rarg(lean_object*, lean_object*, lean_object*);
+uint8_t l_instDecidablePredNatTurn__fst(lean_object*);
+lean_object* l_List_range(lean_object*);
+lean_object* l_List_lengthTRAux___rarg(lean_object*, lean_object*);
+LEAN_EXPORT lean_object* l_moves__from__strats___rarg___boxed(lean_object*, lean_object*, lean_object*, lean_object*);
+LEAN_EXPORT lean_object* l___private_Games_gameLib__fixfix_Zermelo_0__Y_match__1_splitter___rarg(lean_object*, lean_object*, lean_object*);
+LEAN_EXPORT lean_object* l___private_Games_gameLib__fixfix_Zermelo_0__Y_match__1_splitter___rarg___boxed(lean_object*, lean_object*, lean_object*);
+LEAN_EXPORT lean_object* l_List_rget(lean_object*);
+LEAN_EXPORT lean_object* l___private_Games_gameLib__fixfix_Zermelo_0__Y_match__1_splitter(lean_object*);
+uint8_t lean_nat_dec_eq(lean_object*, lean_object*);
+LEAN_EXPORT lean_object* l_List_rget___rarg(lean_object*, lean_object*);
+lean_object* l_History__on__turn___rarg(lean_object*, lean_object*, lean_object*, lean_object*, lean_object*, lean_object*);
+LEAN_EXPORT lean_object* l_moves__from__strats___rarg(lean_object*, lean_object*, lean_object*, lean_object*);
+lean_object* lean_nat_sub(lean_object*, lean_object*);
+lean_object* l_List_reverse___rarg(lean_object*);
+lean_object* lean_nat_add(lean_object*, lean_object*);
+LEAN_EXPORT lean_object* l_List_rget___rarg(lean_object* x_1, lean_object* x_2) {
+_start:
+{
+lean_object* x_3; lean_object* x_4; lean_object* x_5; lean_object* x_6; lean_object* x_7; lean_object* x_8; 
+x_3 = lean_unsigned_to_nat(0u);
+x_4 = l_List_lengthTRAux___rarg(x_1, x_3);
+x_5 = lean_unsigned_to_nat(1u);
+x_6 = lean_nat_sub(x_4, x_5);
+lean_dec(x_4);
+x_7 = lean_nat_sub(x_6, x_2);
+lean_dec(x_6);
+x_8 = l_List_get___rarg(x_1, x_7);
+return x_8;
+}
+}
+LEAN_EXPORT lean_object* l_List_rget(lean_object* x_1) {
+_start:
+{
+lean_object* x_2; 
+x_2 = lean_alloc_closure((void*)(l_List_rget___rarg___boxed), 2, 0);
+return x_2;
+}
+}
+LEAN_EXPORT lean_object* l_List_rget___rarg___boxed(lean_object* x_1, lean_object* x_2) {
+_start:
+{
+lean_object* x_3; 
+x_3 = l_List_rget___rarg(x_1, x_2);
+lean_dec(x_2);
+lean_dec(x_1);
+return x_3;
+}
+}
+LEAN_EXPORT lean_object* l_Hist__from__moves___rarg(lean_object* x_1, lean_object* x_2) {
+_start:
+{
+lean_object* x_3; lean_object* x_4; lean_object* x_5; lean_object* x_6; 
+x_3 = l_List_range(x_2);
+x_4 = l_List_reverse___rarg(x_3);
+x_5 = lean_box(0);
+x_6 = l_List_mapTR_loop___rarg(x_1, x_4, x_5);
+return x_6;
+}
+}
+LEAN_EXPORT lean_object* l_Hist__from__moves(lean_object* x_1) {
+_start:
+{
+lean_object* x_2; 
+x_2 = lean_alloc_closure((void*)(l_Hist__from__moves___rarg), 2, 0);
+return x_2;
+}
+}
+LEAN_EXPORT lean_object* l_moves__from__strats___rarg(lean_object* x_1, lean_object* x_2, lean_object* x_3, lean_object* x_4) {
+_start:
+{
+lean_object* x_5; lean_object* x_6; lean_object* x_7; lean_object* x_8; uint8_t x_9; 
+x_5 = lean_ctor_get(x_1, 0);
+lean_inc(x_3);
+lean_inc(x_2);
+x_6 = l_History__on__turn___rarg(x_5, lean_box(0), lean_box(0), x_2, x_3, x_4);
+x_7 = lean_unsigned_to_nat(1u);
+x_8 = lean_nat_add(x_4, x_7);
+x_9 = l_instDecidablePredNatTurn__fst(x_8);
+lean_dec(x_8);
+if (x_9 == 0)
+{
+lean_object* x_10; 
+lean_dec(x_2);
+x_10 = lean_apply_3(x_3, x_6, lean_box(0), lean_box(0));
+return x_10;
+}
+else
+{
+lean_object* x_11; 
+lean_dec(x_3);
+x_11 = lean_apply_3(x_2, x_6, lean_box(0), lean_box(0));
+return x_11;
+}
+}
+}
+LEAN_EXPORT lean_object* l_moves__from__strats(lean_object* x_1, lean_object* x_2) {
+_start:
+{
+lean_object* x_3; 
+x_3 = lean_alloc_closure((void*)(l_moves__from__strats___rarg___boxed), 4, 0);
+return x_3;
+}
+}
+LEAN_EXPORT lean_object* l_moves__from__strats___rarg___boxed(lean_object* x_1, lean_object* x_2, lean_object* x_3, lean_object* x_4) {
+_start:
+{
+lean_object* x_5; 
+x_5 = l_moves__from__strats___rarg(x_1, x_2, x_3, x_4);
+lean_dec(x_4);
+lean_dec(x_1);
+return x_5;
+}
+}
+LEAN_EXPORT lean_object* l___private_Games_gameLib__fixfix_Zermelo_0__Y_match__1_splitter___rarg(lean_object* x_1, lean_object* x_2, lean_object* x_3) {
+_start:
+{
+lean_object* x_4; uint8_t x_5; 
+x_4 = lean_unsigned_to_nat(0u);
+x_5 = lean_nat_dec_eq(x_1, x_4);
+if (x_5 == 0)
+{
+lean_object* x_6; lean_object* x_7; lean_object* x_8; 
+x_6 = lean_unsigned_to_nat(1u);
+x_7 = lean_nat_sub(x_1, x_6);
+x_8 = lean_apply_1(x_3, x_7);
+return x_8;
+}
+else
+{
+lean_dec(x_3);
+lean_inc(x_2);
+return x_2;
+}
+}
+}
+LEAN_EXPORT lean_object* l___private_Games_gameLib__fixfix_Zermelo_0__Y_match__1_splitter(lean_object* x_1) {
+_start:
+{
+lean_object* x_2; 
+x_2 = lean_alloc_closure((void*)(l___private_Games_gameLib__fixfix_Zermelo_0__Y_match__1_splitter___rarg___boxed), 3, 0);
+return x_2;
+}
+}
+LEAN_EXPORT lean_object* l___private_Games_gameLib__fixfix_Zermelo_0__Y_match__1_splitter___rarg___boxed(lean_object* x_1, lean_object* x_2, lean_object* x_3) {
+_start:
+{
+lean_object* x_4; 
+x_4 = l___private_Games_gameLib__fixfix_Zermelo_0__Y_match__1_splitter___rarg(x_1, x_2, x_3);
+lean_dec(x_2);
+lean_dec(x_1);
+return x_4;
+}
+}
+lean_object* initialize_Init(uint8_t builtin, lean_object*);
+lean_object* initialize_Games_gameLib__fixfix_Termination(uint8_t builtin, lean_object*);
+static bool _G_initialized = false;
+LEAN_EXPORT lean_object* initialize_Games_gameLib__fixfix_Zermelo(uint8_t builtin, lean_object* w) {
+lean_object * res;
+if (_G_initialized) return lean_io_result_mk_ok(lean_box(0));
+_G_initialized = true;
+res = initialize_Init(builtin, lean_io_mk_world());
+if (lean_io_result_is_error(res)) return res;
+lean_dec_ref(res);
+res = initialize_Games_gameLib__fixfix_Termination(builtin, lean_io_mk_world());
+if (lean_io_result_is_error(res)) return res;
+lean_dec_ref(res);
+return lean_io_result_mk_ok(lean_box(0));
+}
+#ifdef __cplusplus
+}
+#endif
