Games/gameLib_fixfix/Termination.lean
@@ -5,14 +5,14 @@ Released under Apache 2.0 license as described in the file LICENSE.
 Author: Yves Jäckle.
 -/
 
-import Games.gameLib_fix.Basic
+import Games.gameLib_fixfix.Basic
 
 
 inductive Game_World.Turn_isWL (g : Game_World α β)
   (f_strat : fStrategy g.init_game_state g.fst_legal g.snd_legal)
   (s_strat : sStrategy g.init_game_state g.fst_legal g.snd_legal) (turn : ℕ) : Prop where
-| wf : g.fst_win_states (g.state_on_turn f_strat s_strat turn) → g.Turn_isWL f_strat s_strat turn
-| ws : g.snd_win_states (g.state_on_turn f_strat s_strat turn) → g.Turn_isWL f_strat s_strat turn
+| wf : g.fst_win_states g.init_game_state (History_on_turn g.init_game_state g.fst_legal g.snd_legal f_strat s_strat turn) → g.Turn_isWL f_strat s_strat turn
+| ws : g.snd_win_states g.init_game_state (History_on_turn g.init_game_state g.fst_legal g.snd_legal f_strat s_strat turn) → g.Turn_isWL f_strat s_strat turn
 
 
 def Symm_Game_World.Turn_isWL (g : Symm_Game_World α β)
@@ -45,15 +45,11 @@ def Symm_Game_World.isWL_wBound (g : Symm_Game_World α β) (T : ℕ): Prop :=
   ∃ turn ≤ T, g.Turn_isWL f_strat s_strat turn
 
 
-def State_from_history_neutral (ini : α ) (f_trans s_trans : α → List β → (β → α)) (f_wins s_wins : α → Prop) (hist : List β) : Prop :=
-  (¬ (f_wins (State_from_history ini f_trans s_trans hist))) ∧ (¬ (s_wins (State_from_history ini f_trans s_trans hist)))
-
-
 
 def Game_World.state_on_turn_neutral (g : Game_World α β)
   (f_strat : fStrategy g.init_game_state g.fst_legal g.snd_legal)
   (s_strat : sStrategy g.init_game_state g.fst_legal g.snd_legal) (turn : ℕ) : Prop :=
-  (¬ (g.fst_win_states (g.state_on_turn f_strat s_strat turn))) ∧ (¬ (g.snd_win_states (g.state_on_turn f_strat s_strat turn)))
+  ¬ g.Turn_isWL f_strat s_strat turn
 
 def Symm_Game_World.state_on_turn_neutral (g : Symm_Game_World α β)
   (f_strat : fStrategy g.init_game_state g.law g.law)
@@ -67,23 +63,12 @@ def Symm_Game.state_on_turn_neutral (g : Symm_Game α β) (turn : ℕ) : Prop :=
   g.toGame.state_on_turn_neutral turn
 
 
-lemma Game_World.state_on_turn_neutral_State_from_history_neutral (g : Game_World α β)
-  (f_strat : fStrategy g.init_game_state g.fst_legal g.snd_legal)
-  (s_strat : sStrategy g.init_game_state g.fst_legal g.snd_legal) (turn : ℕ) :
-  g.state_on_turn_neutral f_strat s_strat turn ↔
-  State_from_history_neutral g.init_game_state g.fst_transition g.snd_transition g.fst_win_states g.snd_win_states
-  (History_on_turn g.init_game_state g.fst_legal g.snd_legal f_strat s_strat turn).val :=
-  by
-  dsimp [Game_World.state_on_turn_neutral, State_from_history_neutral]
-  rw [Game_World.state_on_turn_State_from_history]
-
-
 def Game.fst_win  {α β : Type _} (g : Game α β) : Prop :=
-  ∃ turn : ℕ, g.fst_win_states (g.state_on_turn turn) ∧
+  ∃ turn : ℕ, g.fst_win_states g.init_game_state (History_on_turn g.init_game_state g.fst_legal g.snd_legal g.fst_strat g.snd_strat turn) ∧
     (∀ t < turn, g.state_on_turn_neutral t)
 
 def Game.snd_win  {α β : Type _} (g : Game α β) : Prop :=
-  ∃ turn : ℕ, g.snd_win_states (g.state_on_turn turn) ∧
+  ∃ turn : ℕ, g.snd_win_states g.init_game_state (History_on_turn g.init_game_state g.fst_legal g.snd_legal g.fst_strat g.snd_strat turn) ∧
     (∀ t < turn, g.state_on_turn_neutral t)
 
 def Symm_Game.fst_win  {α β : Type _} (g : Symm_Game α β) : Prop :=
@@ -115,23 +100,50 @@ inductive Game_World.has_WL (g : Game_World α β) : Prop where
 def Symm_Game_World.has_WL (g : Symm_Game_World α β) := g.toGame_World.has_WL
 
 
+def State_from_history_neutral (ini : α ) (f_wins s_wins : α → List β → Prop) (hist : List β) : Prop :=
+  (¬ (f_wins ini hist)) ∧ (¬ (s_wins ini hist))
+
+
+lemma Game_World.state_on_turn_neutral_State_from_history_neutral (g : Game_World α β)
+  (f_strat : fStrategy g.init_game_state g.fst_legal g.snd_legal)
+  (s_strat : sStrategy g.init_game_state g.fst_legal g.snd_legal) (turn : ℕ) :
+  g.state_on_turn_neutral f_strat s_strat turn ↔
+  State_from_history_neutral g.init_game_state g.fst_win_states g.snd_win_states
+  (History_on_turn g.init_game_state g.fst_legal g.snd_legal f_strat s_strat turn).val :=
+  by
+  dsimp [Game_World.state_on_turn_neutral, State_from_history_neutral]
+  rw [← not_or, not_iff_not]
+  constructor
+  · intro h
+    cases' h with F S
+    · left ; exact F
+    · right ; exact S
+  · intro h
+    cases' h with F S
+    · apply Game_World.Turn_isWL.wf ; exact F
+    · apply Game_World.Turn_isWL.ws ; exact S
+
+
+
 
 -- # Coherent end
 
 structure Game_World.coherent_end (g : Game_World α β) : Prop where
-  em : ∀ s : α, ¬ (g.fst_win_states s ∧ g.snd_win_states s)
-  fst : ∀ hist, Hist_legal g.init_game_state g.fst_legal g.snd_legal hist → (g.fst_win_states (State_from_history g.init_game_state g.fst_transition g.snd_transition hist) →
+  em : ∀ hist, Hist_legal g.init_game_state g.fst_legal g.snd_legal hist → ¬ (g.fst_win_states g.init_game_state hist ∧ g.snd_win_states g.init_game_state hist)
+  fst : ∀ hist, Hist_legal g.init_game_state g.fst_legal g.snd_legal hist → (g.fst_win_states g.init_game_state hist →
           ∀ act, ((Turn_fst (hist.length+1) → g.fst_legal g.init_game_state hist act) ∧ (Turn_snd (hist.length+1) → g.snd_legal g.init_game_state hist act)) →
-            g.fst_win_states ((State_from_history g.init_game_state g.fst_transition g.snd_transition (act :: hist))))
-  snd : ∀ hist, Hist_legal g.init_game_state g.fst_legal g.snd_legal hist → (g.snd_win_states (State_from_history g.init_game_state g.fst_transition g.snd_transition hist) →
+            g.fst_win_states g.init_game_state (act :: hist))
+  snd : ∀ hist, Hist_legal g.init_game_state g.fst_legal g.snd_legal hist → (g.snd_win_states g.init_game_state hist →
           ∀ act, ((Turn_fst (hist.length+1) → g.fst_legal g.init_game_state hist act) ∧ (Turn_snd (hist.length+1) → g.snd_legal g.init_game_state hist act)) →
-            g.snd_win_states ((State_from_history g.init_game_state g.fst_transition g.snd_transition (act :: hist))))
+            g.snd_win_states g.init_game_state (act :: hist))
+
+
 
 
 lemma Game_World.coherent_end_all_fst (g : Game_World α β)  (h : g.coherent_end)
-  (hist : List β) (hw : g.fst_win_states (State_from_history g.init_game_state g.fst_transition g.snd_transition hist))
+  (hist : List β) (hw : g.fst_win_states g.init_game_state hist)
   (future : List β) (fleg : Hist_legal g.init_game_state g.fst_legal g.snd_legal (future ++ hist)) :
-  g.fst_win_states (State_from_history g.init_game_state g.fst_transition g.snd_transition (future ++ hist)) :=
+  g.fst_win_states g.init_game_state (future ++ hist) :=
   by
   induction' future with x l ih
   · apply hw
@@ -150,9 +162,9 @@ lemma Game_World.coherent_end_all_fst (g : Game_World α β)  (h : g.coherent_en
 
 
 lemma Game_World.coherent_end_all_snd (g : Game_World α β)  (h : g.coherent_end)
-  (hist : List β) (hw : g.snd_win_states (State_from_history g.init_game_state g.fst_transition g.snd_transition hist))
+  (hist : List β) (hw : g.snd_win_states g.init_game_state hist)
   (future : List β) (fleg : Hist_legal g.init_game_state g.fst_legal g.snd_legal (future ++ hist)) :
-  g.snd_win_states (State_from_history g.init_game_state g.fst_transition g.snd_transition (future ++ hist)) :=
+  g.snd_win_states g.init_game_state (future ++ hist) :=
   by
   induction' future with x l ih
   · apply hw
@@ -172,18 +184,16 @@ lemma Game_World.coherent_end_all_snd (g : Game_World α β)  (h : g.coherent_en
 
 lemma Game_World.coherent_end_for_starts (g : Game_World α β) (hg : g.coherent_end) :
   ∀ (f_strat : fStrategy g.init_game_state g.fst_legal g.snd_legal) (s_strat : sStrategy g.init_game_state g.fst_legal g.snd_legal) (t : ℕ),
-    (g.fst_win_states (g.state_on_turn f_strat s_strat t) → g.fst_win_states (g.state_on_turn f_strat s_strat (t+1))) ∧
-      (g.snd_win_states (g.state_on_turn f_strat s_strat t) → g.snd_win_states (g.state_on_turn f_strat s_strat (t+1))) :=
+    (g.fst_win_states g.init_game_state (History_on_turn g.init_game_state g.fst_legal g.snd_legal f_strat s_strat t) → g.fst_win_states g.init_game_state (History_on_turn g.init_game_state g.fst_legal g.snd_legal f_strat s_strat (t+1))) ∧
+      (g.snd_win_states g.init_game_state (History_on_turn g.init_game_state g.fst_legal g.snd_legal f_strat s_strat t) → g.snd_win_states g.init_game_state (History_on_turn g.init_game_state g.fst_legal g.snd_legal f_strat s_strat (t+1))) :=
   by
   intro f_strat s_strat t
   constructor
   · intro fw
-    rw [g.state_on_turn_State_from_history]
     dsimp [History_on_turn]
     split_ifs with T
     · apply hg.fst _ (History_on_turn g.init_game_state g.fst_legal g.snd_legal f_strat s_strat t).prop.1
-      · rw [← g.state_on_turn_State_from_history]
-        exact fw
+      · exact fw
       · constructor
         · intro T'
           apply (f_strat (History_on_turn g.init_game_state g.fst_legal g.snd_legal f_strat s_strat t).val T' (History_on_turn g.init_game_state g.fst_legal g.snd_legal f_strat s_strat t).prop.1).prop
@@ -192,8 +202,7 @@ lemma Game_World.coherent_end_for_starts (g : Game_World α β) (hg : g.coherent
           exfalso
           exact no T
     · apply hg.fst _ (History_on_turn g.init_game_state g.fst_legal g.snd_legal f_strat s_strat t).prop.1
-      · rw [← g.state_on_turn_State_from_history]
-        exact fw
+      · exact fw
       · constructor
         · intro no
           rw [(History_on_turn g.init_game_state g.fst_legal g.snd_legal f_strat s_strat t).prop.2, Turn_fst_iff_not_snd] at no
@@ -202,12 +211,10 @@ lemma Game_World.coherent_end_for_starts (g : Game_World α β) (hg : g.coherent
         · intro T'
           apply (s_strat (History_on_turn g.init_game_state g.fst_legal g.snd_legal f_strat s_strat t).val T' (History_on_turn g.init_game_state g.fst_legal g.snd_legal f_strat s_strat t).prop.1).prop
   · intro fw
-    rw [g.state_on_turn_State_from_history]
     dsimp [History_on_turn]
     split_ifs with T
     · apply hg.snd _ (History_on_turn g.init_game_state g.fst_legal g.snd_legal f_strat s_strat t).prop.1
-      · rw [← g.state_on_turn_State_from_history]
-        exact fw
+      · exact fw
       · constructor
         · intro T'
           apply (f_strat (History_on_turn g.init_game_state g.fst_legal g.snd_legal f_strat s_strat t).val T' (History_on_turn g.init_game_state g.fst_legal g.snd_legal f_strat s_strat t).prop.1).prop
@@ -216,8 +223,7 @@ lemma Game_World.coherent_end_for_starts (g : Game_World α β) (hg : g.coherent
           exfalso
           exact no T
     · apply hg.snd _ (History_on_turn g.init_game_state g.fst_legal g.snd_legal f_strat s_strat t).prop.1
-      · rw [← g.state_on_turn_State_from_history]
-        exact fw
+      · exact fw
       · constructor
         · intro no
           rw [(History_on_turn g.init_game_state g.fst_legal g.snd_legal f_strat s_strat t).prop.2, Turn_fst_iff_not_snd] at no
@@ -228,8 +234,8 @@ lemma Game_World.coherent_end_for_starts (g : Game_World α β) (hg : g.coherent
 
 lemma Game_World.coherent_end_all_for_strats (g : Game_World α β)  (h : g.coherent_end)
   (f_strat : fStrategy g.init_game_state g.fst_legal g.snd_legal) (s_strat : sStrategy g.init_game_state g.fst_legal g.snd_legal) (t n : ℕ) :
-  (g.fst_win_states (g.state_on_turn f_strat s_strat t) → g.fst_win_states (g.state_on_turn f_strat s_strat (t+n))) ∧
-    (g.snd_win_states (g.state_on_turn f_strat s_strat t) → g.snd_win_states (g.state_on_turn f_strat s_strat (t+n))) :=
+  (g.fst_win_states g.init_game_state (History_on_turn g.init_game_state g.fst_legal g.snd_legal f_strat s_strat t) → g.fst_win_states g.init_game_state (History_on_turn g.init_game_state g.fst_legal g.snd_legal f_strat s_strat (t+n))) ∧
+    (g.snd_win_states g.init_game_state (History_on_turn g.init_game_state g.fst_legal g.snd_legal f_strat s_strat t) → g.snd_win_states g.init_game_state (History_on_turn g.init_game_state g.fst_legal g.snd_legal f_strat s_strat (t+n))) :=
   by
   replace h := g.coherent_end_for_starts h
   constructor
@@ -249,11 +255,11 @@ lemma Game_World.coherent_end_all_for_strats (g : Game_World α β)  (h : g.cohe
 
 
 lemma Game.coherent_end_fst_win (g : Game α β) (hg : g.coherent_end)
-  (main : ∃ turn : ℕ, g.fst_win_states (g.state_on_turn turn)) :
+  (main : ∃ turn : ℕ, g.fst_win_states g.init_game_state (History_on_turn g.init_game_state g.fst_legal g.snd_legal g.fst_strat g.snd_strat turn)) :
   g.fst_win :=
   by
   obtain ⟨t,fw⟩ := main
-  let S : Set Nat := {n : Nat | g.fst_win_states (g.state_on_turn n)}
+  let S : Set Nat := {n : Nat | g.fst_win_states g.init_game_state (History_on_turn g.init_game_state g.fst_legal g.snd_legal g.fst_strat g.snd_strat n)}
   obtain ⟨m,mdef,mm⟩ := WellFounded.wellFounded_iff_has_min.mp Nat.lt_wfRel.wf S (by use t ; apply fw)
   use m
   constructor
@@ -261,21 +267,20 @@ lemma Game.coherent_end_fst_win (g : Game α β) (hg : g.coherent_end)
   · intro n nlm
     unfold state_on_turn_neutral Game_World.state_on_turn_neutral
     by_contra con
-    simp_rw [not_and_or,not_not] at con
     cases' con with con con
     · apply mm n con nlm
     · replace con := (g.coherent_end_all_for_strats hg g.fst_strat g.snd_strat n (m - n)).2 con
       rw [← Nat.add_sub_assoc (le_of_lt nlm), Nat.add_sub_self_left] at con
-      apply hg.em _ ⟨mdef,con⟩
+      apply hg.em _ (History_on_turn g.init_game_state g.fst_legal g.snd_legal g.fst_strat g.snd_strat m).prop.1 ⟨(mdef),con⟩
 
 
 
 lemma Game.coherent_end_snd_win (g : Game α β) (hg : g.coherent_end)
-  (main : ∃ turn : ℕ, g.snd_win_states (g.state_on_turn turn)) :
+  (main : ∃ turn : ℕ, g.snd_win_states g.init_game_state (History_on_turn g.init_game_state g.fst_legal g.snd_legal g.fst_strat g.snd_strat turn)) :
   g.snd_win :=
   by
   obtain ⟨t,fw⟩ := main
-  let S : Set Nat := {n : Nat | g.snd_win_states (g.state_on_turn n)}
+  let S : Set Nat := {n : Nat | g.snd_win_states g.init_game_state (History_on_turn g.init_game_state g.fst_legal g.snd_legal g.fst_strat g.snd_strat n)}
   obtain ⟨m,mdef,mm⟩ := WellFounded.wellFounded_iff_has_min.mp Nat.lt_wfRel.wf S (by use t ; apply fw)
   use m
   constructor
@@ -283,32 +288,13 @@ lemma Game.coherent_end_snd_win (g : Game α β) (hg : g.coherent_end)
   · intro n nlm
     unfold state_on_turn_neutral Game_World.state_on_turn_neutral
     by_contra con
-    simp_rw [not_and_or,not_not] at con
     cases' con with con con
     · replace con := (g.coherent_end_all_for_strats hg g.fst_strat g.snd_strat n (m - n)).1 con
       rw [← Nat.add_sub_assoc (le_of_lt nlm), Nat.add_sub_self_left] at con
-      apply hg.em _ ⟨con, mdef⟩
+      apply hg.em _ (History_on_turn g.init_game_state g.fst_legal g.snd_legal g.fst_strat g.snd_strat m).prop.1 ⟨con,mdef⟩
     · apply mm n con nlm
 
 
 
 
-
--- TODO : Refactor ↓
-#exit
-
-def Symm_Game_World.coherent_end (g : Symm_Game_World α β) : Prop :=
-  ∀ (f_strat : fStrategy g.init_game_state g.law g.law) (s_strat : sStrategy g.init_game_state g.law g.law) (t : ℕ),
-    g.win_states (g.state_on_turn f_strat s_strat t) → g.win_states (g.state_on_turn f_strat s_strat (t+1))
-
-
-lemma Symm_Game_World.coherent_end_all (g : Symm_Game_World α β)  (h : g.coherent_end)
-  (f_strat : fStrategy g.init_game_state g.law g.law) (s_strat : sStrategy g.init_game_state g.law g.law) (t n : ℕ) :
-  g.win_states (g.state_on_turn f_strat s_strat t) → g.win_states (g.state_on_turn f_strat s_strat (t+n)) :=
-  by
-  intro H
-  induction' n with n ih
-  · dsimp
-    exact H
-  · apply h _ _
-    exact ih
+def Symm_Game_World.coherent_end (g : Symm_Game_World α β) : Prop := g.toGame_World.coherent_end
