Games/gameLib_fixfix/Stealing.lean
@@ -5,7 +5,7 @@ Author: Yves Jäckle.
 -/
 
 
-
+import Games.gameLib_fixfix.Zermelo
 
 
 #exit
